

Good work

SMA 2480 - COMPLEX ANALYSIS REVISION

Ex.

1. Given $z_1 = 3+4i$ and $z_2 = 5+3i$. Compute:

(i) $z_1 \cdot z_2^{-1}$

$z_2^{-1} = ?$ but $z_2 \cdot z_2^{-1} = 1$ --- (i)

where $z_2 = 5+3i$ --- (ii)

z_2^{-1} from (i) $= z_2^{-1} = \frac{1}{z_2}$

$z_2^{-1} = \frac{1}{5+3i}$

$5+3i$

so $z_1 \cdot z_2^{-1} = \frac{3+4i}{5+3i} \cdot \frac{5-3i}{5-3i}$

$z_1 \cdot z_2^{-1} = \frac{3(5-3i) + 4i(5-3i)}{5^2 - 9}$

$z_1 \cdot z_2^{-1} = \frac{15-9i+20i-12}{34}$

$z_1 \cdot z_2^{-1} = \frac{27+11i}{34} = \frac{27}{34} + \frac{11}{34}i$

(ii) $z_2 \cdot z_1^{-1}$

given $z_1 \cdot z_1^{-1} = 1$

$z_1^{-1} = \frac{1}{z_1}$ where $z_1 = 3+4i$

$z_1^{-1} = \frac{1}{3+4i}$

so $z_2 \cdot z_1^{-1} = \frac{5+3i}{3+4i}$

$z_2 \cdot z_1^{-1} = \frac{5+3i}{3+4i} \cdot \frac{3-4i}{3-4i} = \frac{5(3-4i) + 3i(3-4i)}{(3+4i)(3-4i)} = \frac{15-20i+9i-12}{25-16}$

$= \frac{3-11i}{25} = \frac{3}{25} - \frac{11}{25}i$

(iii) $z_1 \cdot z_2$

$$(3+4i)(5+3i)$$

where $z_1 = 3+4i$

$$3(3+4i) + 4i(3+4i)$$

$$\text{so } z_1 \cdot z_2 = (3+4i)^2$$

$$9 + 12i + 12i - 16$$

$$= 9 - 16$$

$$= 24i$$

$$= -7$$

2. Show that $z_1 \cdot z_2 = z_2 \cdot z_1$

Solving L.H.S

$$z_1 \cdot z_2 = (3+4i)(5+3i)$$

$$= 3(5+3i) + 4i(5+3i)$$

$$= 15 + 9i + 20i - 12$$

$$= 3 + 29i$$

Solving R.H.S

$$z_2 \cdot z_1 = (5+3i)(3+4i)$$

$$= 5(3+4i) + 3i(3+4i)$$

$$= 15 + 20i + 9i - 12$$

$$= 3 + 29i$$

R.H.S = L.H.S = $3 + 29i$ so $z_1 \cdot z_2 = z_2 \cdot z_1$ (associative law)

PART 2: DIVISION OF COMPLEX NUMBERS

Exercise

$$(i) \frac{3+4i}{1-2i} \cdot \frac{1+2i}{1+2i} = \frac{3+4i}{1-2i} \cdot \frac{1+2i}{1^2 - (-2)^2} = \frac{3(1+2i) + 4i(1+2i)}{1^2 - (-2)^2}$$

$$1-2i \cdot 1+2i$$

$$1-2i$$

$$1+2i$$

$$1^2 - (-2)^2$$

$$= \frac{3+6i+4i-8}{5} = \frac{10i-5}{5}$$

$$5$$

$$5$$

$$= \frac{2i-1}{1}$$

$$(ii) \frac{2i+4}{3i-7} \cdot \frac{3i+7}{3i+7} = \frac{2i+4}{3i-7} \cdot \frac{3i+7}{(3i)^2 - (-7)^2}$$

$$3i-7$$

$$3i-7$$

$$3i+7$$

$$\frac{2i(3i+7) + 4(3i+7)}{3^2 - (-7)^2}$$

$$= 9 - 49$$

$$= \frac{-6+14i+12i+28}{-58} = \frac{22+26i}{-58} = \frac{-22}{58} - \frac{26i}{58}$$

$$= 58$$

$$= 58$$

$$= 58$$

$$= 58$$